Postulated preservation theorem; Moved additional has_type conditions from SN branch to here.

src/PlutusIR/Semantics/Static/Typing.v
@@ -58,6 +58,54 @@ Reserved Notation "Delta ',,' Gamma '|-ok_b' b" (at level 101, b at level 0, no 
 
 Local Open Scope list_scope.
 
+(* TODO: Do we really need bound variables? *)
+Definition freshUnwrapIFix (F : ty) : string :=
+  "a" ++ String.concat EmptyString (FreeVars.Ty.ftv F).
+
+
+Definition unwrapIFixFresh (F : ty) (K : kind) (T : ty) : ty :=
+  let b := freshUnwrapIFix F in 
+ (Ty_App (Ty_App F (Ty_Lam b K (Ty_IFix F (Ty_Var b)))) T).
+
+(* TODO: See also Theorems/Weakening
+*)
+Lemma weakening : forall T T2 K X Δ,
+      ~ In X (FreeVars.Ty.ftv T) ->
+      Δ |-* T : K ->
+      ((X, T2)::Δ) |-* T : K.
+Proof.
+Admitted.
+
+Lemma unwrapIFixFresh_ftv_helper F :
+  ~ In (freshUnwrapIFix F) (FreeVars.Ty.ftv F).
+Admitted.
+
+Lemma unwrapIFixFresh__well_kinded F K T Δ :
+  Δ |-* F : (Kind_Arrow (Kind_Arrow K Kind_Base) (Kind_Arrow K Kind_Base)) ->
+  Δ |-* T : K ->
+  Δ |-* (unwrapIFixFresh F K T) : Kind_Base.
+Proof.
+  intros.
+  unfold unwrapIFix.
+  eapply K_App with (K1 := K); auto.
+  eapply K_App with (K1 := Kind_Arrow K Kind_Base); auto.
+  eapply K_Lam.
+  eapply K_IFix with (K := K); auto.
+  - remember (freshUnwrapIFix F) as X.
+    constructor.
+    simpl.
+    rewrite String.eqb_refl.
+    reflexivity.
+  - remember (freshUnwrapIFix F) as x.
+    (* Now weaken *)
+    eapply weakening with (Δ := Δ); auto.
+    unfold List.inclusion.
+    (* By definition of freshUnwrapIFix *)
+    subst.
+    apply unwrapIFixFresh_ftv_helper.
+Qed.
+
+
 (* 
 Should have
 drop_ty_var "s" (("x", Ty_Bool) :: ("x", Ty_Var "s") :: ("x", Ty_Int) :: nil) = nil
@@ -80,8 +128,9 @@ Definition drop_ty_var X (Γ : list (string * ty)) : list (string * ty) :=
 
 Inductive has_type : list (string * kind) -> list (string * ty) -> term -> ty -> Prop :=
   (* Simply typed lambda caclulus *)
-  | T_Var : forall Γ Δ x T Tn,
+  | T_Var : forall Γ Δ x T Tn K,
       lookup x Γ = Coq.Init.Datatypes.Some T ->
+      Δ |-* T : K ->
       normalise T Tn ->
       Δ ,, Γ |-+ (Var x) : Tn
   | T_LamAbs : forall Δ Γ x T1 t T2n T1n,
@@ -99,6 +148,7 @@ Inductive has_type : list (string * kind) -> list (string * ty) -> term -> ty ->
       Δ ,, Γ |-+ (TyAbs X K t) : (Ty_Forall X K Tn)
   | T_TyInst : forall Δ Γ t1 T2 T1n X K2 T0n T2n,
       Δ ,, Γ |-+ t1 : (Ty_Forall X K2 T1n) ->
+      ((X, K2)::Δ) |-* T1n : Kind_Base -> (* Richard: Added *)
       Δ |-* T2 : K2 ->
       normalise T2 T2n ->
       normalise (substituteTCA X T2n T1n) T0n ->
@@ -109,13 +159,13 @@ Inductive has_type : list (string * kind) -> list (string * ty) -> term -> ty ->
       normalise T Tn ->
       Δ |-* F : (Kind_Arrow (Kind_Arrow K Kind_Base) (Kind_Arrow K Kind_Base)) ->
       normalise F Fn ->
-      normalise (unwrapIFix Fn K Tn) T0n ->
+      normalise (unwrapIFixFresh Fn K Tn) T0n ->
       Δ ,, Γ |-+ M : T0n ->
       Δ ,, Γ |-+ (IWrap F T M) : (Ty_IFix Fn Tn)
   | T_Unwrap : forall Δ Γ M Fn K Tn T0n,
       Δ ,, Γ |-+ M : (Ty_IFix Fn Tn) ->
       Δ |-* Tn : K ->
-      normalise (unwrapIFix Fn K Tn) T0n ->
+      normalise (unwrapIFixFresh Fn K Tn) T0n ->
       Δ ,, Γ |-+ (Unwrap M) : T0n
   (* Additional constructs *)
   | T_Constant : forall Δ Γ T a,
@@ -124,16 +174,19 @@ Inductive has_type : list (string * kind) -> list (string * ty) -> term -> ty ->
       T = lookupBuiltinTy f ->
       normalise T Tn ->
       Δ ,, Γ |-+ (Builtin f) : Tn
-  | T_Error : forall Δ Γ S T Tn,
-      Δ |-* T : Kind_Base ->
-      normalise T Tn ->
-      Δ ,, Γ |-+ (Error S) : Tn
+  | T_Error : forall Δ Γ S Sn,
+      Δ |-* S : Kind_Base ->
+      normalise S Sn ->
+      Δ ,, Γ |-+ (Error S) : Sn
   (** Let-bindings
       Note: The rules for let-constructs differ significantly from the paper definitions
       because we had to adapt the typing rules to the compiler implementation of type checking.
       Reference: The Haskell module PlutusIR.TypeCheck.Internal in the
       iohk/plutus/plutus-core/plutus-ir project.
   **)
+
+(* TODO: Check for changes in Strong normalisation branches to typing rules*)
+
   | T_Let : forall Δ Γ bs t Tn Δ' Γ' bsGn,
       Δ' = flatten (map binds_Delta bs) ++ Δ ->
       map_normalise (flatten (map binds_Gamma bs)) bsGn ->
