src/PlutusIR/Semantics/TypeSafety/Preservation.v
@@ -1,0 +1,117 @@
+Require Import PlutusCert.PlutusIR.Semantics.Dynamic.Bigstep.
+Require Import PlutusCert.PlutusIR.Semantics.Static.Typing.
+Require Import PlutusCert.PlutusIR.Semantics.TypeSafety.SubstitutionPreservesTyping.
+Require Import PlutusCert.PlutusIR.Semantics.TypeSafety.TypeLanguage.Preservation.
+Require Import PlutusCert.PlutusIR.Semantics.Static.Theorems.UniqueTypes.
+Require Import PlutusCert.PlutusIR.Semantics.Static.Theorems.ContextInvariance.AFI.
+(* SubstituteT behaves as substituteTCA when substituting closed types *)
+Lemma closed__substituteT_CA : 
+  forall X U T,
+    Ty.closed U ->
+    substituteTCA X U T = substituteT X U T.
+Proof.
+Admitted.
+
+(* Term language type preservation under evaluation/reduction*)
+Theorem eval__type_preservation : forall t T v k,
+    nil ,, nil |-+ t : T -> (* TODO: closed terms?*)
+    t =[k]=> v ->
+    nil ,, nil |-+ v : T.
+Proof.
+    intros t T v k Ht Hbs.
+    generalize dependent T.
+    induction Hbs; intros.
+    - (* E_LamAbs *)
+      exact Ht.
+    - (* E_Apply *)
+      apply IHHbs3.
+      inversion Ht; subst.
+      apply IHHbs1 in H5.
+      inversion H5; subst.
+      apply substitution_preserves_typing__Term with (U := T1n) (Un := T1n).
+      + auto. 
+      + apply normalisation__stable'__normal.
+        eapply normalise_to_normal; eauto.
+      + apply IHHbs2; auto.
+    - (* E_TyAbs *)
+      exact Ht.
+    - (* E_TyInst *)
+      apply IHHbs2.
+      inversion Ht; subst.
+      apply IHHbs1 in H2.
+      inversion H2; subst.
+      apply substA_preserves_typing__Term__value with (T := T1n) (K := K2).
+      + auto.
+      + auto.
+      + assert ((substituteTCA X0 T2n T1n) = (substituteT X0 T2n T1n)).
+        {
+          apply closed__substituteT_CA.
+          auto.
+          (* By T2 well-kinded in empty environment
+            and normalise preserves kinding *)
+          admit.
+        }
+        rewrite H in H9.
+
+        auto.
+        subst.
+        auto.
+         (* relation of normalise and substituteT
+        *)
+        admit.
+    - (* E_IWrap *)
+      inversion Ht; subst.
+      eapply T_IWrap; eauto. (* Through IHHbs*)
+    - (* E_Unwrap *)
+      inversion Ht; subst.
+      apply IHHbs in H1.
+      inversion H1; subst.
+      assert (K0 = K).
+      {
+        apply (TypeLanguage.Preservation.preservation _ _ _ _ H7) in H10.
+        eapply unique_kinds; eauto.
+      }
+      subst.
+      apply (normalisation__deterministic _ _ _ H5) in H13.
+      subst.
+      auto.
+    - (* E_Constant*)
+      exact Ht.
+    - (* E_Constr_nil *)
+      exact Ht.
+    - (* E_Constr_cons *)
+      
+      admit.
+      (* TODO: No typing rules for constr?*)
+    - (* E_Builtin *)
+      exact Ht.
+    - (* E_Apply_Builtin_Partial *)
+      inversion Ht; subst.
+      inversion H0; subst.
+      + admit.
+      + (* Hmm need some induction *)
+        admit.
+      + (* Some induction *)
+        admit.
+    - (* E_TyInst_Builtin_Partial *)
+      admit.
+    - (* E_Apply_Builtin_Full *)
+      admit.
+    - (* E_TyInst_Builtin_Full *)
+      admit.
+    - (* E_Error *)
+      exact Ht.
+    - (* E_Error_Apply1 *)
+
+      (* TODO: Error rule was changed to allow
+        type checking completeness to go through,
+        but that does no longer work for 
+        preservation now.
+        *)
+
+      inversion Ht; subst.
+      
+      apply IHHbs in H4.
+      
+
+Admitted.
